Addition on ℕ can be substituted and canceled over `≤`

Lean4Axiomatic/AbstractAlgebra.lean
@@ -11,16 +11,6 @@ def forHand {α : Sort u} {β : Sort v} : Hand → (α → α → β) → (α �
 | Hand.L => id
 | Hand.R => flip
 
-class Commutative {α : Type u} [EqvOp α] (f : α → α → α) where
-  comm {x y : α} : f x y ≃ f y x
-
-export Commutative (comm)
-
-instance
-    {α : Type u} [EqvOp α] (f : α → α → α) [Commutative f]
-    : Swap f (· ≃ ·) where
-  swap := comm
-
 class Substitutive
     {α : Sort u} {β : Sort v}
     (f : α → β) (rα : outParam (α → α → Prop)) (rβ : β → β → Prop) where
@@ -29,48 +19,69 @@ class Substitutive
 export Substitutive (subst)
 
 class SubstitutiveForHand
-    (hand : Hand) {α : Sort u} {β : Sort v}
-    (f : α → α → β) (rα : outParam (α → α → Prop)) (rβ : β → β → Prop) where
+    (hand : Hand) {α : Sort u} {β : Sort v} (f : α → α → β)
+    (rα : outParam (α → α → Prop)) (rβ : β → β → Prop) where
   subst₂
     {x₁ x₂ y : α} : rα x₁ x₂ → rβ (forHand hand f x₁ y) (forHand hand f x₂ y)
 
 export SubstitutiveForHand (subst₂)
 
-def substL
-    {α : Sort u} {β : Sort v} {f : α → α → β}
-    {rα : α → α → Prop} {rβ : β → β → Prop}
-    [inst : SubstitutiveForHand Hand.L f rα rβ]  {x₁ x₂ y : α}
-    : rα x₁ x₂ → rβ (f x₁ y) (f x₂ y) := subst₂ (hand := Hand.L)
-
-def substR
-    {α : Sort u} {β : Sort v} {f : α → α → β}
-    {rα : α → α → Prop} {rβ : β → β → Prop}
-    [SubstitutiveForHand Hand.R f rα rβ]  {x₁ x₂ y : α}
-    : rα x₁ x₂ → rβ (f y x₁) (f y x₂) := subst₂ (hand := Hand.R)
-
-def substR_from_substL_swap
-    {α : Sort u} {β : Sort v} {f : α → α → β}
-    {rα : α → α → Prop} {rβ : β → β → Prop}
-    [Refl rβ] [Trans rβ] [Swap f rβ] [SubstitutiveForHand Hand.L f rα rβ]
-    : SubstitutiveForHand Hand.R f rα rβ := by
-  constructor
-  intro x₁ x₂ y (_ : rα x₁ x₂)
-  show rβ (f y x₁) (f y x₂)
-  calc
-    rβ _ (f y x₁) := Refl.refl
-    rβ _ (f x₁ y) := Swap.swap
-    rβ _ (f x₂ y) := AA.substL ‹rα x₁ x₂›
-    rβ _ (f y x₂) := Swap.swap
+abbrev substL := @subst₂ Hand.L
+abbrev substR := @subst₂ Hand.R
 
 class Substitutive₂
     {α : Sort u} {β : Sort v}
     (f : α → α → β) (rα : α → α → Prop) (rβ : β → β → Prop)
     where
-  substitutiveL : SubstitutiveForHand Hand.L f rα rβ
-  substitutiveR : SubstitutiveForHand Hand.R f rα rβ
+  [substitutiveL : SubstitutiveForHand Hand.L f rα rβ]
+  [substitutiveR : SubstitutiveForHand Hand.R f rα rβ]
 
 attribute [instance] Substitutive₂.substitutiveL
 attribute [instance] Substitutive₂.substitutiveR
+
+class Commutative {α : Sort u} {β : Sort v} [EqvOp β] (f : α → α → β) where
+  comm {x y : α} : f x y ≃ f y x
+
+export Commutative (comm)
+
+instance
+    {α : Type u} {β : Type v} {f : α → α → β} {rel : β → β → Prop}
+    [EqvOp β] [Commutative f] [Relation.Refl rel]
+    [SubstitutiveForHand Hand.R rel (· ≃ ·) (· → ·)]
+    : Swap f rel where
+  swap := by
+    intro x y
+    show rel (f x y) (f y x)
+    have : rel (f x y) (f x y) := Eqv.refl
+    exact substR (rβ := (· → ·)) comm ‹rel (f x y) (f x y)›
+
+def substR_from_substL_swap
+    {α : Sort u} {β : Sort v} {f : α → α → β}
+    {rα : α → α → Prop} {rβ : β → β → Prop}
+    [Trans rβ] [Swap f rβ] [SubstitutiveForHand Hand.L f rα rβ]
+    : SubstitutiveForHand Hand.R f rα rβ := by
+  constructor
+  intro x₁ x₂ y (_ : rα x₁ x₂)
+  show rβ (f y x₁) (f y x₂)
+  calc
+    rβ (f y x₁) (f x₁ y) := Swap.swap
+    rβ (f x₁ y) (f x₂ y) := AA.substL ‹rα x₁ x₂›
+    rβ (f x₂ y) (f y x₂) := Swap.swap
+
+instance {α : Sort u} [EqvOp α]
+    : SubstitutiveForHand Hand.L (α := α) (· ≃ ·) (· ≃ ·) (· → ·) := by
+  constructor
+  intro x₁ x₂ y (_ : x₁ ≃ x₂) (_ : x₁ ≃ y)
+  show x₂ ≃ y
+  exact Eqv.trans (Eqv.symm ‹x₁ ≃ x₂›) ‹x₁ ≃ y›
+
+instance {α : Sort u} [EqvOp α]
+    : SubstitutiveForHand Hand.R (α := α) (· ≃ ·) (· ≃ ·) (· → ·) :=
+  substR_from_substL_swap
+
+instance {α : Sort u} [EqvOp α]
+    : Substitutive₂ (α := α) (· ≃ ·) (· ≃ ·) (· → ·) :=
+  Substitutive₂.mk
 
 instance neq.substL
     {α : Sort u} [EqvOp α]
@@ -80,12 +91,42 @@ instance neq.substL
   show False
   apply ‹x₁ ≄ y›
   show x₁ ≃ y
-  exact Eqv.trans ‹x₁ ≃ x₂› ‹x₂ ≃ y›   
+  exact Eqv.trans ‹x₁ ≃ x₂› ‹x₂ ≃ y›
 
 instance
     {α : Sort u} [EqvOp α] : Substitutive₂ (α := α) (· ≄ ·) (· ≃ ·) (· → ·)
     where
   substitutiveL := inferInstance
   substitutiveR := substR_from_substL_swap
-  
+
+class Cancellative
+    (hand : Hand) {α : Sort u} {β : Sort v}
+    (f : α → α → β) (rα : outParam (α → α → Prop)) (rβ : β → β → Prop) where
+  cancel
+    {x y₁ y₂ : α} : rβ (forHand hand f x y₁) (forHand hand f x y₂) → rα y₁ y₂
+
+export Cancellative (cancel)
+
+abbrev cancelL := @cancel Hand.L
+abbrev cancelR := @cancel Hand.R
+
+class Cancellative₂
+    {α : Sort u} {β : Sort v}
+    (f : α → α → β) (rα : outParam (α → α → Prop)) (rβ : β → β → Prop) where
+  [cancellativeL : Cancellative Hand.L f rα rβ]
+  [cancellativeR : Cancellative Hand.R f rα rβ]
+
+def cancelR_from_cancelL
+    {α : Sort u} {β : Sort v}
+    {f : α → α → β} {rα : α → α → Prop} {rβ : β → β → Prop}
+    [EqvOp β] [Commutative f] [Substitutive₂ rβ (· ≃ ·) (· → ·)]
+    [Cancellative Hand.L f rα rβ]
+    : Cancellative Hand.R f rα rβ := by
+  constructor
+  intro x y₁ y₂ (hyp : rβ (f y₁ x) (f y₂ x))
+  show rα y₁ y₂
+  have : rβ (f x y₁) (f y₂ x) := AA.substL (rβ := (· → ·)) AA.comm hyp
+  have : rβ (f x y₁) (f x y₂) := AA.substR (rβ := (· → ·)) AA.comm this
+  exact AA.cancelL this
+
 end AA
